updated rtl for fdel

week-03/week3_stack_height.v
@@ -1312,6 +1312,8 @@ Qed.
 
 (* *** End of List Length *** *)
 
+(* Start of depth functions *)
+
 Definition test_depth (candidate : arithmetic_expression -> nat) : bool :=
   let ae1 := (Literal 1) in
   let ae2 := (Plus
@@ -1404,7 +1406,9 @@ Proof.
   fold_unfold_tactic depth.
 Qed.
 
-(* ***** *)
+(* End of depth functions *)
+
+(* Start of depth left functions *)
 
 Definition test_depth_left (candidate : arithmetic_expression -> nat) : bool :=
   let ae1 := (Literal 1) in
@@ -1458,7 +1462,9 @@ Proof.
   fold_unfold_tactic depth_left.
 Qed.
 
-(* ***** *)
+(* End of depth left functions *)
+
+(* Start of depth right functions *)
 
 Definition test_depth_right (candidate : arithmetic_expression -> nat) : bool :=
   let ae1 := (Literal 1) in
@@ -1512,7 +1518,10 @@ Proof.
   fold_unfold_tactic depth_right.
 Qed.
 
-(* ***** *)
+
+(* End of depth right functions *)
+
+(* Start of fetch_decode_execute with height ltr functions *)
 
 Definition eqb_option (V : Type) (eqb_V : V -> V -> bool) (ov1 ov2 : option V) : bool :=
   match ov1 with
@@ -1714,38 +1723,41 @@ Definition run_height_ltr (tp : target_program) : expressible_value * nat :=
 
 Compute (test_run_height_ltr run_height_ltr).
 
-(* ***** *)
+(* End of fetch_decode_execute with height ltr functions *)
 
-Definition test_decode_execute_height_rtl (candidate : byte_code_instruction -> data_stack -> nat -> result_of_decoding_and_execution_height) : bool :=
+(* Start of fetch_decode_execute with height rtl functions *)
+
+Definition test_decode_execute_height_rtl (candidate : byte_code_instruction -> data_stack  -> result_of_decoding_and_execution_height) : bool :=
   (eqb_result_of_decoding_and_execution_height
-     (candidate (PUSH 42) (1 :: 2 :: 3 :: nil) 3)
+     (candidate (PUSH 42) (1 :: 2 :: 3 :: nil))
      (OK_h (42 :: 1 :: 2 :: 3 :: nil) 4))
   &&
     (eqb_result_of_decoding_and_execution_height
-       (candidate (PUSH 42) (1 :: 2 :: 3 :: nil) 10)
-       (OK_h (42 :: 1 :: 2 :: 3 :: nil) 10))
+       (candidate (PUSH 42) (1 :: 2 :: 3 :: nil))
+       (OK_h (42 :: 1 :: 2 :: 3 :: nil) 4))
   &&
     (eqb_result_of_decoding_and_execution_height
-       (candidate ADD (1 :: 2 :: 3 :: nil) 10)
-       (OK_h (3 :: 3 :: nil) 10 ))
+       (candidate ADD (1 :: 2 :: 3 :: nil))
+       (OK_h (3 :: 3 :: nil) 3 ))
   &&
     (eqb_result_of_decoding_and_execution_height
-       (candidate SUB (2 :: 3 :: 3 :: nil) 10)
+       (candidate SUB (2 :: 3 :: 3 :: nil))
        (KO_h "numerical underflow: -1"))
   &&
     (eqb_result_of_decoding_and_execution_height
-       (candidate SUB (3 :: 2 :: 3 :: nil) 10)
-       (OK_h (1 :: 3 :: nil) 10 )).
+       (candidate SUB (3 :: 2 :: 3 :: nil))
+       (OK_h (1 :: 3 :: nil) 3)).
 
-Definition decode_execute_height_rtl (bci : byte_code_instruction) (ds : data_stack) (mh : nat) : result_of_decoding_and_execution_height :=
+Definition decode_execute_height_rtl (bci : byte_code_instruction)
+  (ds : data_stack) : result_of_decoding_and_execution_height :=
   match bci with
-  | PUSH n => OK_h (n :: ds) (max (S (list_length nat ds)) mh)
+  | PUSH n => OK_h (n :: ds) (S (list_length nat ds))
   | ADD =>
       match ds with
       | nil => KO_h "ADD: stack underflow"
       | n1 :: ds' =>
           match ds' with
-          | n2 :: ds'' => OK_h ((n1 + n2) :: ds'') mh
+          | n2 :: ds'' => OK_h ((n1 + n2) :: ds'') (list_length nat ds)
           | nil => KO_h "ADD: stack underflow"
           end
       end
@@ -1759,7 +1771,7 @@ Definition decode_execute_height_rtl (bci : byte_code_instruction) (ds : data_st
               | true =>
                   KO_h (String.append "numerical underflow: -" (string_of_nat (n2 - n1)))
               | false =>
-                  OK_h ((n1 - n2) :: ds'') mh
+                  OK_h ((n1 - n2) :: ds'') (list_length nat ds)
               end
           | nil => KO_h "SUB: stack underflow"
           end
@@ -1768,37 +1780,37 @@ Definition decode_execute_height_rtl (bci : byte_code_instruction) (ds : data_st
 
 Compute test_decode_execute_height_rtl decode_execute_height_rtl.
 
-Definition test_fetch_decode_execute_loop_height_rtl (candidate : (list byte_code_instruction) -> data_stack -> nat -> result_of_decoding_and_execution_height) :=
+Definition test_fetch_decode_execute_loop_height_rtl (candidate : (list byte_code_instruction) -> data_stack  -> result_of_decoding_and_execution_height) :=
   (eqb_result_of_decoding_and_execution_height
-     (candidate (PUSH 42 :: PUSH 21 :: nil) (1 :: 2 :: 3 :: nil) 3)
+     (candidate (PUSH 42 :: PUSH 21 :: nil) (1 :: 2 :: 3 :: nil))
      (OK_h (21 :: 42 :: 1 :: 2 :: 3 :: nil) 5))
   &&
     (eqb_result_of_decoding_and_execution_height
-       (candidate (ADD :: ADD :: nil) (1 :: 2 :: 3 :: nil) 3)
+       (candidate (ADD :: ADD :: nil) (1 :: 2 :: 3 :: nil))
        (OK_h (6 :: nil) 3))
   &&
     (eqb_result_of_decoding_and_execution_height
-       (candidate (SUB :: nil) (3 :: 2 :: nil) 2)
+       (candidate (SUB :: nil) (3 :: 2 :: nil))
        (OK_h (1 :: nil) 2 ))
   &&
     (eqb_result_of_decoding_and_execution_height
-       (candidate (SUB :: SUB :: nil) (4 :: 3 :: 2 :: nil) 2)
+       (candidate (SUB :: SUB :: nil) (4 :: 3 :: 2 :: nil))
        (KO_h "numerical underflow: -1"))
   &&
     (eqb_result_of_decoding_and_execution_height
        (candidate
-          (PUSH 1 :: PUSH 2 :: ADD :: PUSH 3 :: ADD :: PUSH 4 :: ADD :: nil) nil 0)
+          (PUSH 1 :: PUSH 2 :: ADD :: PUSH 3 :: ADD :: PUSH 4 :: ADD :: nil) nil)
        (OK_h (10 :: nil) 2)).
 
-Fixpoint fetch_decode_execute_loop_height_rtl (bcis : list byte_code_instruction) (ds : data_stack) (mh : nat): result_of_decoding_and_execution_height :=
+Fixpoint fetch_decode_execute_loop_height_rtl (bcis : list byte_code_instruction) (ds : data_stack) : result_of_decoding_and_execution_height :=
   match bcis with
-  | nil => OK_h ds mh
+  | nil => OK_h ds (list_length nat ds)
   | bci :: bcis' =>
-      match decode_execute_height_rtl bci ds mh with
+      match decode_execute_height_rtl bci ds with
       | OK_h ds' mh' =>
-          match fetch_decode_execute_loop_height_rtl bcis' ds' mh' with
+          match fetch_decode_execute_loop_height_rtl bcis' ds' with
           | OK_h ds'' mh'' =>
-              OK_h ds'' mh''
+              OK_h ds'' (max (list_length nat ds) mh'')
           | KO_h s =>
               KO_h s
           end                 
@@ -1809,10 +1821,9 @@ Fixpoint fetch_decode_execute_loop_height_rtl (bcis : list byte_code_instruction
 Compute (test_fetch_decode_execute_loop_height_rtl fetch_decode_execute_loop_height_rtl).
 
 Lemma fold_unfold_fetch_decode_execute_loop_height_rtl_nil :
-  forall (ds: data_stack)
-         (mh : nat),
-    fetch_decode_execute_loop_height_rtl nil ds mh =
-      OK_h ds mh.
+  forall (ds: data_stack),
+    fetch_decode_execute_loop_height_rtl nil ds =
+    OK_h ds (list_length nat ds).
 Proof.
   fold_unfold_tactic fetch_decode_execute_loop_height_rtl.
 Qed.
@@ -1820,19 +1831,18 @@ Qed.
 Lemma fold_unfold_fetch_decode_execute_loop_height_rtl_cons :
   forall (bci : byte_code_instruction)
          (bcis' : list byte_code_instruction)
-         (ds : data_stack)
-         (mh ch : nat),
-    fetch_decode_execute_loop_height_rtl (bci :: bcis') ds mh =
-      match decode_execute_height_rtl bci ds mh with
-      | OK_h ds' mh' =>
-          match fetch_decode_execute_loop_height_rtl bcis' ds' mh' with
-          | OK_h ds'' mh'' =>
-              OK_h ds'' mh''
-          | KO_h s =>
-              KO_h s
-          end             
-      | KO_h s => KO_h s
-      end.
+         (ds : data_stack),
+    fetch_decode_execute_loop_height_rtl (bci :: bcis') ds =
+    match decode_execute_height_rtl bci ds with
+    | OK_h ds' mh' =>
+        match fetch_decode_execute_loop_height_rtl bcis' ds' with
+        | OK_h ds'' mh'' =>
+            OK_h ds'' (max (list_length nat ds) mh'')
+        | KO_h s =>
+            KO_h s
+        end                 
+    | KO_h s => KO_h s
+    end.
 Proof.
   fold_unfold_tactic fetch_decode_execute_loop_height_rtl.
 Qed.
@@ -1857,7 +1867,7 @@ Definition test_run_height_rtl (candidate : target_program -> expressible_value 
 Definition run_height_rtl (tp : target_program) : expressible_value * nat :=
   match tp with
   | Target_program bcis =>
-    match fetch_decode_execute_loop_height_rtl bcis nil 0 with
+    match fetch_decode_execute_loop_height_rtl bcis nil with
     | OK_h ds mh =>
         match ds with
         | nil => (Expressible_msg "no result on the data stack", 0)
@@ -1873,7 +1883,9 @@ Definition run_height_rtl (tp : target_program) : expressible_value * nat :=
 
 Compute (test_run_height_rtl run_height_rtl).
 
-(* ***** *)
+(* End of fetch_decode_execute with height rtl functions *)
+
+(* Sanity check that run_height_ltr works for balanced trees of Plus operators *)
 
 Compute (let ae1 := (Plus
                        (Plus (Literal 1) (Literal 2))
